Termination is porven

SATsolver/Experiment/DPLL/backtrack.lean
@@ -1,6 +1,7 @@
 import SATsolver.Experiment.Relations.Theories
+import SATsolver.Experiment.DPLL.misc
 
-def backtrack (t : Trail)(wf : ∃ a ∈ t, a.decidedP) : Trail :=
+def backtrack (t : Trail)(wf : ∃ a ∈ t, a.decidedP)(twf : t.wf) : Trail :=
   have : t ≠ [] := by
     intro contra
     simp[contra] at wf
@@ -9,6 +10,10 @@ def backtrack (t : Trail)(wf : ∃ a ∈ t, a.decidedP) : Trail :=
     match a with
     | .decided l => (ALit.deduced l.negate)::as
     | .deduced _ =>
+      have aswf : Trail.wf as := by
+        simp[Trail.wf, Trail.names] at twf ⊢
+        simp[twf]
+        exact twf.2.2
       have : (∃ a ∈ as, a.decidedP) := by
         obtain ⟨ a, amem, adec ⟩ := wf
         rw[ALit.dec_is_dec] at adec
@@ -16,10 +21,10 @@ def backtrack (t : Trail)(wf : ∃ a ∈ t, a.decidedP) : Trail :=
         simp [ha] at amem
         exists a
         simp[ha, amem, ALit.decidedP]
-      backtrack as this
+      backtrack as this aswf
 
-theorem backtrack_lemma {hd tl : Trail}{a : ALit}{wf: ∃ e ∈ (hd++a::tl), e.decidedP} :
-  (∀ e ∈ hd, ¬ e.decidedP) → a.decidedP → backtrack (hd++a::tl) wf = (ALit.deduced a.lit.negate)::tl := by
+theorem backtrack_lemma {hd tl : Trail}{a : ALit}{wf: ∃ e ∈ (hd++a::tl), e.decidedP}{twf : (hd++a::tl).wf} :
+  (∀ e ∈ hd, ¬ e.decidedP) → a.decidedP → backtrack (hd++a::tl) wf twf = (ALit.deduced a.lit.negate)::tl := by
   intro hhd ha
   cases a
   case deduced => simp[ALit.decidedP] at ha
@@ -44,3 +49,25 @@ theorem backtrack_lemma {hd tl : Trail}{a : ALit}{wf: ∃ e ∈ (hd++a::tl), e.d
       case deduced =>
         simp[backtrack]
         exact ih hhd2
+
+
+theorem bck_preserves_twf {t : Trail}{f : Formula}
+{wf : ∃ a ∈ t, a.decidedP}{twf : t.wf}{tf : ∀ n ∈ t.names, n ∈ f.names} :
+(backtrack t wf twf).wf ∧ ∀ n ∈ (backtrack t wf twf).names, n ∈ f.names := by
+  obtain ⟨ hd, tl, a, heq, ha, hhd ⟩  := exists_split_on_prop ALit.decidedP t wf
+  rw[heq] at wf twf
+  have bck_lemma : backtrack (hd++a::tl) wf twf = (ALit.deduced a.lit.negate)::tl := backtrack_lemma hhd ha
+  have names : Trail.names (a :: tl) = Trail.names (ALit.deduced a.lit.negate :: tl) := by
+    simp[Trail.names, ALit.name, Lit.name_name_negate, ALit.lit]
+    cases a
+    all_goals simp
+  simp[heq, bck_lemma, ←names] at ⊢
+  constructor
+  case left =>
+    have wf := Trail.wf_append twf
+    simp[Trail.wf] at wf
+    simp[←names, Trail.wf, wf]
+  case right =>
+    intro n nmem
+    rw[heq, Trail.names_append] at tf
+    exact tf n (by simp[nmem])
