SATsolver/Experiment/Data/Trail.lean
@@ -20,12 +20,28 @@ theorem mem_name_exists_mem {t : Trail}{n : Nat} :
   n ∈ t.names → ∃ a ∈ t, a.name = n := by
   simp[names]
 
+theorem names_append(hd tl : Trail):
+  (hd++tl).names = hd.names++tl.names := by
+  simp[names]
+
+theorem names_cons (hd: ALit)(tl : Trail):
+  Trail.names (hd::tl) = hd.name::tl.names := by
+  simp[names]
+
 def unseen (t : Trail)(n : Nat) : Prop := n ∉ t.names
 
 instance : DecidableRel unseen :=
   fun t n => inferInstanceAs (Decidable (n ∉ t.names))
 
-def wf (t : Trail) : Prop := t.names.Nodup
+def wf (t : Trail) : Prop := t.names.Nodup ∧ 0 ∉ t.names
 
-instance : DecidablePred Trail.wf :=
-  fun t => List.nodupDecidable (t.names)
+instance : DecidablePred Trail.wf := by
+  intro t
+  simp[wf]
+  apply instDecidableAnd
+
+def wf_append{hd tl : Trail}:
+  (hd++tl).wf → hd.wf ∧ tl.wf := by
+  simp[wf, names_append, List.nodup_append]
+  intro hdNodup tlNodup nodup nozerohd nozerotl
+  simp[hdNodup, tlNodup, nozerohd, nozerotl]
