SATsolver/Experiment/DPLL/decide.lean
@@ -2,3 +2,24 @@ import SATsolver.Experiment.Relations.Theories
 
 def dec (l : Lit)(t : Trail)(_ : t ¿ l): Trail :=
   ALit.decided l :: t
+
+theorem dec_preserves_wf{l : Lit}{t : Trail}{lud : t ¿ l}{f : Formula}
+  {fwf : f.wf}{twf : t.wf ∧ ∀ n ∈ t.names, n ∈ f.names}:
+  l.name ∈ f.names → (dec l t lud).wf ∧ ∀ n ∈ (dec l t lud).names, n ∈ f.names := by
+  intro lmem
+  simp[Undecided.ud] at lud
+  constructor
+  case left =>
+    have : 0 ≠ l.name := by
+      intro contra
+      simp[Formula.wf, Clause.wf] at fwf
+      simp[Formula.names] at lmem
+      obtain ⟨ c, cmem, cname ⟩ := lmem
+      simp[←contra, (fwf c cmem).2.2] at cname
+    simp[Trail.wf, dec, Trail.names_cons, ALit.name, lud, twf.1.1, twf.1.2, this]
+  case right =>
+    intro n nmem
+    simp[dec] at nmem
+    cases nmem
+    case head => simp[ALit.name, lmem]
+    case tail tail => exact twf.2 n tail
