SATsolver/Experiment/DPLL/impl.lean
@@ -1,7 +1,9 @@
 import SATsolver.Experiment.Relations.Theories
 import SATsolver.Experiment.DPLL.distance
 
-def internal (t : Trail)(f : Formula)(wf : f ≠ []): Bool :=
+
+
+def internal (t : Trail)(f : Formula)(v : Variables)(vz : v ≠ 0)(wf : f.wf ∧ v.wf f)(twf : t.wf ∧ ∀ n ∈ t.names, n ∈ f.names): Bool :=
   if sat : decide (t ⊨ f) then
     true
   else if con : decide (t ⊭ f) then
@@ -10,7 +12,7 @@ def internal (t : Trail)(f : Formula)(wf : f ≠ []): Bool :=
         simp[ALit.decidedP_iff_decidedB] at anyDec
         obtain ⟨ a, amem, adec ⟩ := anyDec
         exists a
-      internal (backtrack t bcwf) f wf
+      internal (backtrack t bcwf twf.1) f v vz wf (bck_preserves_twf (tf := twf.2))
     else false
   else
     let copt := f.find? (fun c => c.unit t)
@@ -23,16 +25,20 @@ def internal (t : Trail)(f : Formula)(wf : f ≠ []): Bool :=
         have := List.find?_some cunit
         simp at this
         exact this
-      internal (propogate t c this) f wf
+      have cmem : c ∈ f := by
+        simp only [copt] at h
+        have := List.get_find?_mem h
+        simp[c, copt, this]
+      internal (propogate t c this) f v vz wf (ppg_preserves_wf cmem (fwf := wf.1) (twf := twf))
     else
       have ud : t¿f := by
         simp at *
         exact Formula.nSatCon_ud sat con
       let copt := (f.find? (t¿·))
-      have : copt.isSome := by
+      have csome : copt.isSome := by
         have := Formula.ud_iff_exists_csUD.mp ud
         simp[copt, this]
-      let c := copt.get this
+      let c := copt.get csome
       have : t ¿ c := by
         have heq : copt = some c := by
           simp[c]
@@ -41,10 +47,10 @@ def internal (t : Trail)(f : Formula)(wf : f ≠ []): Bool :=
         simp at this
         exact this
       let lopt := (c.find? (t¿·))
-      have : lopt.isSome := by
+      have lsome : lopt.isSome := by
         have := Clause.ud_exists_lUd this
         simp[lopt, this]
-      let l := lopt.get this
+      let l := lopt.get lsome
       have : t ¿ l := by
         have heq : lopt = some l := by
           simp[l]
@@ -52,12 +58,37 @@ def internal (t : Trail)(f : Formula)(wf : f ≠ []): Bool :=
         have := List.find?_some heq
         simp at this
         exact this
-      internal (dec l t this) f wf
-termination_by distance t f wf
+      have lmem : l.name ∈ f.names := by
+        simp[Formula.names]
+        exists c
+        constructor
+        case left =>
+          simp only [copt] at csome
+          have := List.get_find?_mem csome
+          simp[c, copt, this]
+        case right =>
+          apply Clause.mem_mem_name
+          simp only[lopt] at lsome
+          have := List.get_find?_mem lsome
+          simp[l, lopt, this]
+      internal (dec l t this) f v vz wf (dec_preserves_wf (fwf := wf.1) (twf := twf) lmem)
+termination_by distance t v vz
 decreasing_by
-  have : f.names.eraseDups.length > t.length := by sorry
+  have : t.length ≤ v := Trail.mem_vwf twf.1 twf.2 wf.2
   exact distance_bc this
-  have : f.names.eraseDups.length > t.length := by sorry
+  have : t.length < v := by
+    simp at sat con
+    have := Trail.ud_vars twf.1 wf.1 wf.2 twf.2 (Formula.nSatCon_ud sat con)
+    simp[Trail.names] at this
+    exact this
   exact distance_prop this
-  have : f.names.eraseDups.length > t.length := by sorry
+  have : t.length < v := by
+    simp at sat con
+    have := Trail.ud_vars twf.1 wf.1 wf.2 twf.2 (Formula.nSatCon_ud sat con)
+    simp[Trail.names] at this
+    exact this
   exact distance_dec this
+
+
+def DPLL(f : Formula)(v : Variables)(vz : v ≠ 0)(wf : f.wf ∧ v.wf f) :=
+  internal [] f v vz wf (by simp[Trail.wf, Trail.names])
