SATsolver/Experiment/DPLL/propogate.lean
@@ -3,3 +3,26 @@ import SATsolver.Experiment.Relations.Theories
 def propogate (t : Trail)(c : Clause)(wf : c.unit t): Trail :=
   let l := c.getunit t wf
   ALit.deduced l :: t
+
+theorem ppg_preserves_wf {t : Trail}{c : Clause}{cu : c.unit t}{f : Formula}
+  {fwf : f.wf}{twf : t.wf ∧ ∀ n ∈ t.names, n ∈ f.names}:
+  c ∈ f → (propogate t c cu).wf ∧ ∀ n ∈ (propogate t c cu).names, n ∈ f.names := by
+  intro cmem
+  have unit_ud : t ¿ c.getunit t cu := Clause.unit_ud
+  have unit_mem : c.getunit t cu ∈ c := Clause.unit_mem
+  have unit_name_mem := Clause.mem_mem_name unit_mem
+  simp[Trail.wf, Undecided.ud, Formula.wf, Clause.wf] at *
+  constructor
+  case left =>
+    have : 0 ≠ (c.getunit t cu).name := by
+      intro contra
+      simp[←contra, (fwf c cmem).2.2] at unit_name_mem
+    simp[propogate, List.nodup_cons, Trail.names_cons, twf, ALit.name, unit_ud, this]
+  case right =>
+    intro n nmem
+    simp[propogate] at nmem
+    cases nmem
+    case head =>
+      have := Formula.mem_memClause_mem_names cmem unit_name_mem
+      simp[ALit.name, this]
+    case tail mem => exact twf.2 n mem
