SATsolver/Experiment/Relations/Theories.lean
@@ -65,3 +65,204 @@ theorem Formula.nSatCon_ud{f : Formula}{t : Trail}:
   have ncCon := ncon c cmem
   have := Clause.nSatCon_ud ncCon ncSat
   exists c
+
+
+theorem length_le_of_nodup_all_le {l : List Nat}{n : Nat}:
+  l.Nodup → 0 ∉ l → (∀ m ∈ l, m ≤ n) → l.length ≤ n := by
+  intro nodup hzero hall
+  induction n generalizing l
+  case zero =>
+    simp
+    false_or_by_contra
+    rename _ => contra
+    obtain ⟨ n, ns, hn ⟩ := List.ne_nil_iff_exists_cons.mp contra
+    subst hn
+    have : n = 0 := by
+      have := hall n (by simp)
+      simp[←Nat.le_zero, this]
+    simp[this] at hzero
+  case succ x ih =>
+    let l' := l.erase (x+1)
+    have nodup' : l'.Nodup := List.Nodup.erase (x+1) nodup
+    have hzero' : 0 ∉ l' := by
+      intro contra
+      have := List.mem_of_mem_erase contra
+      contradiction
+    have hall' : ∀ (m : Nat), m ∈ l' → m ≤ x := by
+      intro y ymem
+      have : y ∈ l := List.mem_of_mem_erase ymem
+      have : y ≤ x + 1 := hall y this
+      simp[l', List.Nodup.mem_erase_iff nodup] at ymem
+      simp[Nat.le_iff_lt_or_eq, ymem.1] at this
+      exact Nat.le_iff_lt_add_one.mpr this
+    have ihc := ih nodup' hzero' hall'
+    by_cases hmem : (x+1) ∈ l
+    case pos =>
+      have : l'.length = l.length - 1 := List.length_erase_of_mem hmem
+      simp[this] at ihc
+      exact ihc
+    case neg =>
+      have : l' = l := List.erase_of_not_mem hmem
+      simp[←this, Nat.le_succ_of_le, ihc]
+
+theorem length_eq_of_nodup_complete_le {l : List Nat}{n : Nat}:
+  l.Nodup → 0 ∉ l → (∀ m ∈ l, m ≤ n) → (∀ m ≤ n, m ∈ l) → l.length = n := by
+  intro nodup hzero hall complete
+  induction n generalizing l
+  case zero =>
+    cases l
+    case nil => simp
+    case cons hd tl =>
+      have : hd ≤ 0 := hall hd (by simp)
+      have : hd = 0 := Nat.le_zero.mp this
+      subst this
+      simp at hzero
+  case succ n ih =>
+    let l' := l.erase (n+1)
+    have nodup' : l'.Nodup := List.Nodup.erase (n+1) nodup
+    have hzero' : 0 ∉ l' := by
+      intro contra
+      have := List.mem_of_mem_erase contra
+      contradiction
+    have hall' : ∀ (m : Nat), m ∈ l' → m ≤ n := by
+      intro y ymem
+      have : y ∈ l := List.mem_of_mem_erase ymem
+      have : y ≤ n + 1 := hall y this
+      simp[l', List.Nodup.mem_erase_iff nodup] at ymem
+      simp[Nat.le_iff_lt_or_eq, ymem.1] at this
+      exact Nat.le_iff_lt_add_one.mpr this
+    have complete' : ∀ (m : Nat), m ≤ n → m ∈ l' := by
+      intro x hmem
+      simp[l', List.Nodup.mem_erase_iff nodup]
+      have := Nat.le_succ_of_le hmem
+      simp[complete x this]
+      intro contra
+      simp[contra] at hmem
+      simp +arith at hmem
+    have ihc := ih nodup' hzero' hall' complete'
+    have hmem : (n+1) ∈ l := complete (n+1) (by simp)
+    have : l'.length = l.length - 1 := List.length_erase_of_mem hmem
+    simp[this] at ihc
+    have : 1 ≤ l.length := by
+      false_or_by_contra
+      rename _ => contra
+      have := Nat.gt_of_not_le contra
+      simp at this
+      simp[this] at hmem
+    simp[← ihc, Nat.sub_add_cancel this]
+
+theorem length_lt_of_nodup_incomplete_le {l : List Nat}{n : Nat}:
+  n ≠ 0 → l.Nodup → 0 ∉ l → (∃ e ≤ n, 0 < e ∧ e ∉ l)→ (∀ m ∈ l, m ≤ n) → l.length < n := by
+  intro neq nodup hzero incopmlete hall
+  induction n generalizing l
+  case zero => contradiction
+  case succ n ih =>
+    let l' := l.erase (n+1)
+    have nodup' : l'.Nodup := List.Nodup.erase (n+1) nodup
+    have hzero' : 0 ∉ l' := by
+      intro contra
+      have := List.mem_of_mem_erase contra
+      contradiction
+    have hall' : ∀ (m : Nat), m ∈ l' → m ≤ n := by
+      intro y ymem
+      have : y ∈ l := List.mem_of_mem_erase ymem
+      have : y ≤ n + 1 := hall y this
+      simp[l', List.Nodup.mem_erase_iff nodup] at ymem
+      simp[Nat.le_iff_lt_or_eq, ymem.1] at this
+      exact Nat.le_iff_lt_add_one.mpr this
+    obtain ⟨ e, hle, h0lt, emem ⟩ := incopmlete
+    cases Nat.lt_or_eq_of_le hle
+    case inl hlt =>
+      have incomplete' : ∃ e, e ≤ n ∧ 0 < e ∧ ¬e ∈ l' := by
+        exists e
+        have : e ≠ n + 1 := Nat.ne_of_lt hlt
+        rw[←List.mem_erase_of_ne this] at emem
+        simp[l', emem, Nat.le_of_lt_add_one, hlt, h0lt]
+      by_cases heq : n = 0
+      case pos =>
+        subst heq
+        simp at hlt
+        simp[hlt] at h0lt
+      case neg =>
+        have ihc := ih heq nodup' hzero' incomplete' hall'
+        by_cases hmem : (n+1) ∈ l
+        case pos =>
+          have : l'.length = l.length - 1 := List.length_erase_of_mem hmem
+          rw[this] at ihc
+          have : 1 ≤ l.length := by
+            false_or_by_contra
+            rename _ => contra
+            have := Nat.gt_of_not_le contra
+            simp at this
+            simp[this] at hmem
+          have := Nat.le_of_lt ihc
+          simp at this
+          cases Nat.lt_or_eq_of_le this
+          case inl this => exact this
+          case inr this => simp[this] at ihc
+        case neg =>
+          have : l' = l := List.erase_of_not_mem hmem
+          simp[←this, Nat.lt_succ_of_lt, ihc]
+    case inr heq =>
+      rw[heq] at emem
+      have heq : l' = l := List.erase_of_not_mem emem
+      have := length_le_of_nodup_all_le nodup' hzero' hall'
+      rw[heq] at this
+      simp[Nat.lt_succ_iff, this]
+
+theorem Variables.ud_not_nil{v : Variables}{t : Trail}{f : Formula}:
+  f.wf → v.wf f → t ¿ f → v ≠ 0 := by
+  simp[Formula.wf, Clause.wf,  Variables.wf, Undecided.ud]
+  intro hall vwf₁ vwf₂ c cmem l lmem lud cud
+  have lcn : l.name ∈ c.names := Clause.mem_mem_name lmem
+  have lfn : l.name ∈ f.names := by
+    exact Formula.mem_memClause_mem_names cmem lcn
+  have vge : l.name ≤ v := vwf₁ l.name lfn
+  have : 0 < l.name := by
+    have := (hall c cmem).2.2
+    by_cases heq : l.name =0
+    case pos => rw[heq] at lcn; contradiction
+    case neg => simp[←Nat.ne_zero_iff_zero_lt, heq]
+  have : 0 < v := Nat.lt_of_lt_of_le this vge
+  simp[Nat.ne_zero_iff_zero_lt, this]
+
+
+theorem Trail.ud_vars{t : Trail}{f : Formula}{v : Variables} :
+  t.wf → f.wf → v.wf f → (∀ n ∈ t.names, n ∈ f.names) → t ¿ f → t.names.length < v := by
+  intro twf fwf vwf htf fud
+  have v_ne_zero := Variables.ud_not_nil fwf vwf fud
+  simp[Trail.wf, Formula.wf, Variables.wf, Undecided.ud] at *
+  have h1 : ∀ n ∈ t.names, n ≤ v := by
+    intro n nmem
+    have : n ∈ f.names := htf n nmem
+    exact vwf.1 n this
+  have h2 : ∃ e, e ≤ v ∧ 0 < e ∧ ¬e ∈ t.names := by
+    obtain ⟨ c, cmem, cud ⟩ := fud
+    obtain ⟨ l, lmem, lud ⟩ :=cud.1
+    exists l.name
+    simp[lud]
+    have cwf : c.wf := fwf c cmem
+    simp[Clause.wf] at cwf
+    by_cases heq : l.name =0
+    case pos =>
+      have := Clause.mem_mem_name lmem
+      simp[heq, cwf] at this
+    case neg =>
+      simp[←Nat.ne_zero_iff_zero_lt, heq]
+      apply vwf.1
+      have := Clause.mem_mem_name lmem
+      exact Formula.mem_memClause_mem_names cmem this
+  exact length_lt_of_nodup_incomplete_le v_ne_zero twf.1 twf.2 h2 h1
+
+
+theorem Trail.mem_vwf {t : Trail}{v : Variables}{f :Formula}:
+  t.wf → (∀ (n : Nat), n ∈ t.names → n ∈ f.names) → v.wf f → t.length ≤ v := by
+  intro twf htf vwf
+  simp[Variables.wf, Trail.wf] at vwf twf
+  have : ∀ (n : Nat), n ∈ t.names → n ≤ v := by
+    intro n nmem
+    have := htf n nmem
+    exact vwf.1 n this
+  have := length_le_of_nodup_all_le twf.1 twf.2 this
+  simp[names] at this
+  exact this
